wip

proof/correctness/Correctness_Hash.ec
@@ -3,10 +3,10 @@ pragma Goals : printall.
 require import AllCore List RealExp IntDiv.
 from Jasmin require import JModel.
 
-require import XMSS_IMPL_PP XMSS_IMPL.
+require import RandomBytes XMSS_IMPL XMSS_IMPL_HOP1.
 require import Address Notation Primitives XMSS_MT_PRF.
 
-require import Array8 Array32 Array64.
+require import Array8 Array32 Array64 Array128.
 (*---*) import NBytes.
 
 require import Utils. (* valid_ptr *)
@@ -16,7 +16,6 @@ pred array32_list_eq (x : W8.t Array32.t) (y : W8.t list) =
 
 axiom hash_ptr (mem : global_mem_t) (ptr inlen : W64.t) :
   array32_list_eq (Hash_ptr ptr inlen) (Hash (mkseq (fun (i : int) => loadW8 mem ((W64.to_uint ptr) + i)) (to_uint inlen))).
-
 
 op addr_to_bytes (a : W32.t Array8.t) : W8.t Array32.t.
 
@@ -34,34 +33,30 @@ axiom prf_equiv (out : W8.t Array32.t, addr : W32.t Array8.t, seed : W8.t Array3
 axiom hash_F_equiv (a : key, b : nbytes) : F a b = Hash (a ++ b).
 
 
-lemma thash_f_correct (_out_ : W8.t Array32.t, _pub_seed_ : W8.t Array32.t, _addr_ : W32.t Array8.t) :
-    equiv [Mp(Syscall).__thash_f ~ Chain.thash :
-      arg{1}=(_out_, _pub_seed_, _addr_) /\ arg{2}=(to_list _out_, _addr_, to_list _pub_seed_) ==>
-       res{2}.`1 = to_list res{1}.`1 /\ res{1}.`2 = res{2}.`2].
-proof.
-proc.
-auto => />.
-- move => &1 &2 * ; split.
-  + admit.
-  + admit.
-- admit.
-qed.
+search Array64.init.
 
-lemma thash_rand_hash (_out : W8.t Array32.t, _in : W8.t Array64.t, _seed : W8.t Array32.t, _addr : W32.t Array8.t) :
-    hoare[Mp(Syscall).__thash_h : 
-      arg = (_out, _in, _seed, _addr) ==> 
-          res.`1 = Array32.of_list witness (rand_hash (to_list _out) (to_list _in) (to_list _seed) _addr).`1].
+op thash_encode (_left _right : W8.t Array32.t) : W8.t Array64.t = 
+    Array64.init (fun (i : int) => if 0 <= i < 32 then _left.[i] else _right.[i-32]).
+
+
+
+lemma thash_rand_hash ( _left _right : W8.t Array32.t, _seed : W8.t Array32.t, _addr : W32.t Array8.t) :
+    equiv[ 
+      M_Hop1(Syscall).__thash_h ~ RandHash.rand_hash : 
+      arg{1}.`2 = (thash_encode _left _right) /\ 
+      arg{1}.`3 = _seed /\ 
+      arg{1}.`4 = _addr /\
+      arg{2} = (to_list _left, to_list _right, to_list _seed, _addr)
+      ==> 
+      res{2}.`1 = to_list res{1}.`1 /\ res{1}.`2 = res{2}.`2
+    ].
 proof.
 proc.
-auto => />.
-- move => &hr H0 addr buf H1. congr. rewrite /rand_hash. admit.
-- while (
-  0 <= to_uint i <= 64
-) ; auto => />.
-    + progress. 
-      * rewrite to_uintD /#.
-      * rewrite to_uintD_small ; smt(@W64).
-    + progress. congr. rewrite /rand_hash. admit.
-    + admit.
+auto => />. move => &1 &2. 
+auto => />. (* simplify before moving to the context *)
+move => addrL bufL *. do split.
+  + admit.
+  + admit.
+admit.
 qed.
 
